Migrate Utilities to ValidPos

correctness/RegexCorrectness/Regex/Matches.lean
@@ -3,84 +3,41 @@ import RegexCorrectness.Regex.Basic
 
 set_option autoImplicit false
 
-open String (Pos Iterator)
+open String (ValidPos ValidPosPlusOne Slice)
 
 namespace Regex.Matches
 
+variable {haystack : String} {self self' : Matches haystack} {slice : Slice}
+
 /--
-The pair of positions returned by `Matches` functions conforms to the spec if and only if:
+The slice returned by `Matches` functions conforms to the spec if and only if:
 
-- the haystack can be split into `l`, `m`, and `r` such that `haystack = l ++ m ++ r`
-- `m` starts after `startPos`.
-- there is a regex match starting at `l`, matching the substring `m`, and ending at `r`
-- the returned substring corresponds to `m`.
+- The start position is valid (i.e., in the range of the haystack)
+- The slice starts after the start position
+- There is a regex match spanning the slice
 -/
-def Spec {re : Regex} (s : re.IsSearchRegex) (haystack : String) (startPos : Pos.Raw) (str : Substring) : Prop :=
-  ∃ it it' groups,
-    it.toString = haystack ∧
-    startPos ≤ it.pos ∧
-    s.expr.Captures it it' groups ∧
-    str = ⟨haystack, it.pos, it'.pos⟩
+def Spec {re : Regex} (s : re.IsSearchRegex) (haystack : String) (startPos : ValidPosPlusOne haystack) (slice : Slice) (eqs : slice.str = haystack) : Prop :=
+  ∃ isValid pos pos' groups,
+    startPos.asValidPos isValid ≤ pos ∧
+    s.expr.Captures pos pos' groups ∧
+    slice.startInclusive = eqs ▸ pos ∧
+    slice.endExclusive = eqs ▸ pos'
 
-def Valid (self : Matches) : Prop :=
-  self.regex.IsSearchRegex ∧ self.currentPos.ValidPlus self.haystack
-
-theorem captures_of_next?_some {self self' : Matches} {s} (h : self.next? = .some (s, self'))
-  (v : self.Valid) :
-  self'.Valid ∧ Spec v.1 self.haystack self.currentPos s := by
-  unfold next? at h
-  split at h
-  next le =>
-    have pos_valid := v.2.valid_of_le le
-    match h' : self.regex.searchNext ⟨self.haystack, self.currentPos⟩ with
-    | none => simp [h'] at h
-    | some matched =>
-      simp [h'] at h
-      have ⟨it, it', groups, eqs, le, c, eq₁, eq₂⟩ := v.1.searchNext_some h' pos_valid
-      simp at eqs
-      refine ⟨?v', it, it', groups, eqs, le, c, ?eq⟩
-      case eq =>
-        simp [Regex.searchNext, Option.bind_eq_some_iff] at h'
-        have ⟨_, _, p₁, _, p₂, _, h'⟩ := h'
-        simp [←h'] at eq₁ eq₂
-        simp [←h.1, ←h', eq₁, eq₂]
-      case v' =>
-        split at h
-        next =>
-          simp [←h.2]
-          have vp : Pos.Raw.ValidPlus it.toString matched.stopPos := c.toString_eq ▸ eq₂ ▸ c.validR.validPlus
-          exact ⟨v.1, eqs ▸ vp⟩
-        next =>
-          simp [←h.2]
-          exact ⟨v.1, String.Pos.Raw.validPlus_of_next_valid pos_valid⟩
-  next => simp at h
-
-theorem regex_eq_of_next?_some {self self' : Matches} {positions : Substring} (h : self.next? = .some (positions, self')) :
+theorem regex_eq_of_next?_some (h : self.next? = .some (slice, self')) :
   self'.regex = self.regex := by
+  grind [next?]
+
+theorem captures_of_next?_some (h : self.next? = .some (slice, self')) (isr : self.regex.IsSearchRegex) :
+  Spec isr haystack self.currentPos slice (self.str_eq_of_next?_some h) := by
   unfold next? at h
   split at h
-  next =>
-    match h' : self.regex.searchNext ⟨self.haystack, self.currentPos⟩ with
-    | none => simp [h'] at h
-    | some matched =>
-      simp [h'] at h
-      split at h <;> simp [←h]
+  next isValid =>
+    split at h
+    next => grind
+    next slice' h' =>
+      simp only [Option.some.injEq, Prod.mk.injEq] at h
+      have ⟨pos, pos', groups, le, c, eq₁, eq₂⟩ := isr.searchNext_some h'
+      exact ⟨isValid, pos, pos', groups, le, c, h.1 ▸ eq₁, h.1 ▸ eq₂⟩
   next => simp at h
-
-theorem haystack_eq_of_next?_some {self self' : Matches} {positions} (h : self.next? = .some (positions, self')) :
-  self'.haystack = self.haystack := by
-  unfold next? at h
-  split at h
-  next =>
-    match h' : self.regex.searchNext ⟨self.haystack, self.currentPos⟩ with
-    | none => simp [h'] at h
-    | some matched =>
-      simp [h'] at h
-      split at h <;> simp [←h]
-  next => simp at h
-
-theorem vaild_matches {re : Regex} (haystack : String) (s : re.IsSearchRegex) :
-  (re.matches haystack).Valid :=
-  ⟨s, haystack.valid_mkIterator.validPlus⟩
 
 end Regex.Matches
