correctness/RegexCorrectness/Regex/Utilities.lean
@@ -4,88 +4,70 @@ import RegexCorrectness.Regex.Captures
 
 set_option autoImplicit false
 
-open String (Pos)
+open String (ValidPos Slice)
 
 namespace Regex
 
-variable {re : Regex} {haystack : String}
+variable {re : Regex} {haystack : String} {slice : Slice}
 
-theorem captures_of_find_some {positions} (h : re.find haystack = .some positions)
-  (s : re.IsSearchRegex) :
-  Matches.Spec s haystack ⟨0⟩ positions := by
-  simp [Regex.find] at h
+theorem find_str_eq_some (h : re.find haystack = .some slice) :
+  slice.str = haystack := by
+  grind [Matches.str_eq_of_next?_some, Option.map_eq_some_iff, find]
+
+theorem captures_of_find_some  (h : re.find haystack = .some slice)
+  (isr : re.IsSearchRegex) :
+  Matches.Spec isr haystack haystack.startValidPosPlusOne slice (find_str_eq_some h) := by
+  simp only [find, Option.map_eq_some_iff, Prod.exists, exists_and_right, exists_eq_right] at h
   have ⟨_, h⟩ := h
-  have v := Captures.valid_captures haystack s
-  exact (Matches.captures_of_next?_some h v).2
+  exact Matches.captures_of_next?_some h isr
 
-theorem captures_of_mem_findAll.go {m : Matches} {accum : Array Substring}
-  (v : m.Valid) (inv : ∀ str ∈ accum, ∃ startPos, Matches.Spec v.1 m.haystack startPos str) :
-  ∀ str ∈ findAll.go m accum, ∃ startPos, Matches.Spec v.1 m.haystack startPos str := by
+theorem captures_of_mem_findAll.go {m : Matches haystack} {accum : Array Slice} (isr : m.regex.IsSearchRegex)
+  (inv : ∀ slice ∈ accum, ∃ startPos eq, Matches.Spec isr haystack startPos slice eq) :
+  ∀ slice ∈ findAll.go haystack m accum, ∃ startPos eq, Matches.Spec isr haystack startPos slice eq := by
   induction m, accum using findAll.go.induct with
-  | case1 m accum positions m' next_some? ih =>
+  | case1 m accum slice m' h ih =>
     -- next match is found
-    rw [findAll.go, next_some?]
-    simp
-    have regex_eq := Matches.regex_eq_of_next?_some next_some?
-    have haystack_eq := Matches.haystack_eq_of_next?_some next_some?
-    simp [regex_eq, haystack_eq] at ih
-
-    have ⟨v', spec⟩ := Matches.captures_of_next?_some next_some? v
-    have inv' (str : Substring) (mem : str ∈ accum ∨ str = positions) : ∃ startPos, Matches.Spec v.1 m.haystack startPos str := by
-      cases mem with
-      | inl mem => exact inv str mem
-      | inr eq => exact ⟨m.currentPos, eq ▸ spec⟩
-    exact ih v' inv'
-  | case2 m accum next_none? =>
+    rw [findAll.go, h]
+    have eq' : m'.regex = m.regex := Matches.regex_eq_of_next?_some h
+    have spec : ∃ startPos eq, Matches.Spec isr haystack startPos slice eq := ⟨_, _, m.captures_of_next?_some h isr⟩
+    grind [Matches.regex_eq_of_next?_some]
+  | case2 m accum h =>
     -- next match is not found
-    rw [findAll.go, next_none?]
-    dsimp
+    rw [findAll.go, h]
     exact inv
 
-theorem captures_of_mem_findAll {positions} (mem : positions ∈ re.findAll haystack)
-  (s : re.IsSearchRegex) :
-  ∃ startPos, Matches.Spec s haystack startPos positions := by
-  simp [Regex.findAll] at mem
-  have v := Matches.vaild_matches haystack s
-  exact captures_of_mem_findAll.go v (by simp) positions mem
+theorem captures_of_mem_findAll (mem : slice ∈ re.findAll haystack) (isr : re.IsSearchRegex) :
+  ∃ startPos eq, Matches.Spec isr haystack startPos slice eq := by
+  dsimp [Regex.findAll] at mem
+  have eq : (re.matches haystack).regex = re := rfl
+  exact captures_of_mem_findAll.go (eq ▸ isr) (by grind) slice mem
 
-theorem captures_of_capture_some {captured} (h : re.capture haystack = .some captured)
-  (s : re.IsSearchRegex) :
-  captured.Spec s haystack ⟨0⟩ := by
+theorem captures_of_capture_some {captured} (h : re.capture haystack = .some captured) (isr : re.IsSearchRegex) :
+  captured.Spec isr haystack haystack.startValidPosPlusOne := by
   simp [Regex.capture] at h
   have ⟨_, h⟩ := h
-  have v := Captures.valid_captures haystack s
-  exact (Captures.captures_of_next?_some h v).2
+  exact Captures.captures_of_next?_some h isr
 
-theorem captures_of_mem_captureAll.go {captures : Captures} {accum : Array CapturedGroups}
-  (v : captures.Valid) (inv : ∀ captured ∈ accum, ∃ startPos, CapturedGroups.Spec v.1 captures.haystack startPos captured) :
-  ∀ captured ∈ captureAll.go captures accum, ∃ startPos, CapturedGroups.Spec v.1 captures.haystack startPos captured := by
+theorem captures_of_mem_captureAll.go {captures : Captures haystack} {accum : Array (CapturedGroups haystack)} (isr : captures.regex.IsSearchRegex)
+  (inv : ∀ captured ∈ accum, ∃ startPos, CapturedGroups.Spec isr haystack startPos captured) :
+  ∀ captured ∈ captureAll.go haystack captures accum, ∃ startPos, CapturedGroups.Spec isr haystack startPos captured := by
   induction captures, accum using captureAll.go.induct with
-  | case1 captures accum groups captures' next?_some ih =>
+  | case1 captures accum groups captures' h ih =>
     -- next capture is found
-    rw [captureAll.go, next?_some]
-    simp
-    have regex_eq := Captures.regex_eq_of_next?_some next?_some
-    have haystack_eq := Captures.haystack_eq_of_next?_some next?_some
-    simp [regex_eq, haystack_eq] at ih
-
-    have ⟨v', spec⟩ := Captures.captures_of_next?_some next?_some v
-    have inv' (captured : CapturedGroups) (mem : captured ∈ accum ∨ captured = groups) : ∃ startPos, CapturedGroups.Spec v.1 captures.haystack startPos captured := by
-      cases mem with
-      | inl mem => exact inv captured mem
-      | inr eq => exact ⟨captures.currentPos, eq ▸ spec⟩
-    exact ih v' inv'
+    rw [captureAll.go, h]
+    -- simp
+    have eq' : captures'.regex = captures.regex := Captures.regex_eq_of_next?_some h
+    have spec : ∃ startPos, CapturedGroups.Spec isr haystack startPos groups := ⟨_, captures.captures_of_next?_some h isr⟩
+    grind
   | case2 captures accum next?_none =>
     -- next capture is not found
     rw [captureAll.go, next?_none]
-    simp
     exact inv
 
-theorem captures_of_mem_captureAll {captured} (mem : captured ∈ re.captureAll haystack)
-  (s : re.IsSearchRegex) :
-  ∃ startPos, CapturedGroups.Spec s haystack startPos captured := by
-  simp [Regex.captureAll] at mem
-  have v := Captures.valid_captures haystack s
-  exact captures_of_mem_captureAll.go v (by simp) captured mem
+theorem captures_of_mem_captureAll {captured} (mem : captured ∈ re.captureAll haystack) (isr : re.IsSearchRegex) :
+  ∃ startPos, CapturedGroups.Spec isr haystack startPos captured := by
+  dsimp [Regex.captureAll] at mem
+  have eq : (re.captures haystack).regex = re := rfl
+  exact captures_of_mem_captureAll.go (eq ▸ isr) (by grind) captured mem
 
 end Regex
